cfrontend/Clight_.v
@@ -760,3 +760,50 @@ Proof.
   eapply external_call_trace_length; eauto.
   eapply external_call_trace_length; eauto.
 Qed.
+
+
+Lemma extcall_invalid p se s q:
+  Smallstep_.at_external ((semantics1 p) se) s q ->
+  ~ valid_query (semantics1 p) se q.
+Proof.
+  intros. inv H. unfold valid_query. cbn.
+  intros [? (i & Hi & Hse)].
+  unfold Genv.find_funct in H0.
+  destruct vf; try congruence.
+  destruct Ptrofs.eq_dec; try congruence.
+  unfold Genv.find_funct_ptr in H0.
+  destruct Genv.find_def eqn: Hdef; try congruence.
+  destruct g eqn: Hg; try congruence. inv H0.
+  unfold globalenv in Hdef. cbn in *.
+  rewrite Genv.find_def_spec in Hdef.
+  destruct Genv.invert_symbol eqn: Hs; try congruence.
+  apply Genv.invert_find_symbol in Hs.
+  unfold Genv.symbol_address in Hse.
+  destruct (Genv.find_symbol se i) eqn: Hxe; try congruence.
+  inv Hse. exploit Genv.find_symbol_injective.
+  apply Hs. apply Hxe. intros ->.
+  unfold footprint_of_program in Hi. rewrite Hdef in Hi.
+  subst f. cbn in *. discriminate Hi.
+Qed.
+
+Lemma initial_state_valid p se s q:
+  Smallstep_.initial_state ((semantics1 p) se) q s ->
+  valid_query (semantics1 p) se q.
+Proof.
+  intros. inv H. clear -H0. unfold valid_query; cbn.
+  unfold Genv.find_funct in H0.
+  destruct vf; try congruence.
+  destruct Ptrofs.eq_dec; try congruence.
+  split. intros X. discriminate X.
+  subst. unfold Genv.find_funct_ptr in H0.
+  destruct Genv.find_def eqn: Hdef; try congruence.
+  destruct g; try congruence. inv H0.
+  unfold globalenv in Hdef; cbn in *.
+  rewrite Genv.find_def_spec in Hdef.
+  destruct Genv.invert_symbol eqn: Hse; try congruence.
+  exists i. split. unfold footprint_of_program.
+  rewrite Hdef. auto.
+  unfold Genv.symbol_address.
+  apply Genv.invert_find_symbol in Hse.
+  rewrite Hse. auto.
+Qed.
